Source/DafnyCore/Verifier/BoogieGenerator.Methods.cs
@@ -548,7 +548,7 @@ namespace Microsoft.Dafny {
       if (!options.Get(CommonOptionBag.ReadsClausesOnMethods)
           || m.IsLemmaLike
           || m.Reads.Expressions.Exists(e => e.E is WildcardExpr)
-          || m.HasConcurrentAttribute) {
+          || m.HasVolatileAttribute) {
         etran = etran.WithReadsFrame(null);
       }
       InitializeFuelConstant(m.tok, builder, etran);
@@ -715,8 +715,18 @@ namespace Microsoft.Dafny {
           if (etran.readsFrame != null) {
             CheckFrameEmpty(m.tok, etran, etran.ReadsFrame(m.tok), builder, desc, null);
           } else {
-            // etran.readsFrame being null indicates the default of reads {}
-            // which is the default for concurrent methods
+            // etran.readsFrame being null indicates the default of reads *,
+            // so this is an automatic failure.
+            builder.Add(Assert(m.tok, Expr.False, desc));
+          }
+        }
+        // Also check that the reads clause == {} if the {:volatile} attribute is present
+        if (m.HasVolatileAttribute) {
+          var desc = new PODesc.ConcurrentFrameEmpty("reads clause");
+          if (etran.readsFrame != null) {
+            CheckFrameEmpty(m.tok, etran, etran.ReadsFrame(m.tok), builder, desc, null);
+          } else {
+            // etran.readsFrame being null means no reads in volatile context
           }
         }
 
@@ -725,7 +735,7 @@ namespace Microsoft.Dafny {
           CheckFrameWellFormed(wfo, m.Mod.Expressions, localVariables, builder, etran);
         });
         // Also check that the modifies clause == {} if the {:concurrent} attribute is present
-        if (m.HasConcurrentAttribute) {
+        if (m.HasConcurrentAttribute || m.HasVolatileAttribute) {
           var desc = new PODesc.ConcurrentFrameEmpty("modifies clause");
           CheckFrameEmpty(m.tok, etran, etran.ModifiesFrame(m.tok), builder, desc, null);
         }
