Source/DafnyCore/Verifier/BoogieGenerator.cs
@@ -4062,7 +4062,7 @@ namespace Microsoft.Dafny {
 
     int projectionFunctionCount = 0;
     private Declaration currentDeclaration;
-    private bool isConcurrent => currentDeclaration is Method {HasConcurrentAttribute: true};
+    private bool isVolatile => currentDeclaration is Method {HasVolatileAttribute: true};
 
 
     // ----- Expression ---------------------------------------------------------------------------
